theories/typing/lib/ghostptrtoken/ghostptrtoken_basic.v
@@ -1,0 +1,139 @@
+From lrust.typing Require Export type.
+From lrust.typing Require Import array_util typing.
+From lrust.typing.lib.ghostptrtoken Require Import ghostptrtoken.
+Set Default Proof Using "Type".
+
+Open Scope nat.
+Implicit Type 𝔄 𝔅: syn_type.
+
+Section ghostptrtoken_basic.
+  Context `{!typeG Σ}.
+
+  Lemma real_big_sepM_ty_shr {𝔄 𝔅} (ty: type 𝔄) (f: 𝔄 → 𝔅)
+    aπm (d: nat) κ tid E L F q :
+    real E L ty f → ↑lftN ⊆ F → lft_ctx -∗ elctx_interp E -∗ llctx_interp L q -∗
+    ([∗ map] l ↦ aπ ∈ aπm, ty.(ty_shr) aπ d κ tid l)
+      ={F}▷=∗ |={F}▷=>^d |={F}=>
+        ⌜∃bm, (fmap f) ∘ mapply aπm = const bm⌝ ∗ llctx_interp L q ∗
+        [∗ map] l ↦ aπ ∈ aπm, ty.(ty_shr) aπ d κ tid l.
+  Proof.
+    setoid_rewrite big_opM_map_to_list.
+    rewrite remove_mapply.
+    iIntros ([_ Rl]?) "#LFT #E L tys". iInduction (map_to_list aπm) as [|] "IH" forall (q)=>/=.
+    { iApply step_fupdN_full_intro. iFrame "L". iPureIntro. unfold compose. rewrite fmap_empty. by exists ∅. }
+    iDestruct "tys" as "[ty tys]". iDestruct "L" as "[L L₊]".
+    iMod (Rl with "LFT E L ty") as "Upd"; [done|].
+    iMod ("IH" with "L₊ tys") as "Upd'". iCombine "Upd Upd'" as "Upd". iIntros "!>!>".
+    iApply (step_fupdN_wand with "Upd"). iIntros "[>(%Eq &$&$) >(%Eq' &$&$)] !%".
+    move: Eq=> [b Eq]. move: Eq'=> [bm Eq']. exists (<[a.1:=b]>bm).
+    fun_ext=>/= π. rewrite fmap_insert. by move: (equal_f Eq π) (equal_f Eq' π)=>/= <-<-.
+  Qed.
+
+  Global Instance token_type_contractive 𝔄 : TypeContractive (ghostptrtoken_ty (𝔄:=𝔄)).
+  Proof.
+    split; [by apply type_lft_morphism_id_like|done| |].
+    - move=>/= > ->*. do 13 (f_contractive || f_equiv). by simpl in *.
+    - intros ?????????????. unfold ty_shr. unfold ghostptrtoken_ty. do 9 (f_contractive || f_equiv). by simpl in *.
+  Qed.
+
+  Global Instance token_send {𝔄} (ty: type 𝔄) : Send ty → Send (ghostptrtoken_ty ty).
+  Proof. move=> ?>/=. by do 13 (f_equiv || move=>?). Qed.
+
+  Global Instance token_sync {𝔄} (ty: type 𝔄) : Sync ty → Sync (ghostptrtoken_ty ty).
+  Proof. move=> ?>/=. by do 9 (f_equiv || move=>?). Qed.
+
+  Lemma token_resolve {𝔄} (ty: type 𝔄) Φ E L :
+    resolve E L ty Φ → resolve E L (ghostptrtoken_ty ty) (mforall Φ).
+  Proof.
+    iIntros (????[|]???) "#LFT #PROPH #E L token //=".
+    iDestruct "token" as (?[->->]) "[↦tys _]". iIntros "!>!>!>".
+    rewrite trans_big_sepM_mt_ty_own. iDestruct "↦tys" as (?) "[↦ tys]".
+    iMod (resolve_big_sepL_ty_own with "LFT PROPH E L tys") as "Upd"; [done..|].
+    iApply (step_fupdN_wand with "Upd").
+    rewrite vec_to_list_map. rewrite vec_to_list_to_vec.
+    setoid_rewrite map_Forall_to_list. setoid_rewrite map_to_list_fmap.
+    unfold lapply. setoid_rewrite <- list_fmap_compose. setoid_rewrite lforall_Forall.
+    setoid_rewrite Forall_fmap. by iIntros "!> H".
+  Qed.
+
+  Lemma token_resolve_just {𝔄} (ty: type 𝔄) E L :
+    resolve E L ty (const True) → resolve E L (ghostptrtoken_ty ty) (const True).
+  Proof. move=> ?. apply resolve_just. Qed.
+
+  Lemma token_real {𝔄 𝔅} (ty: type 𝔄) (f: 𝔄 → 𝔅) E L :
+    real E L ty f → real (𝔅:=fmapₛ _) E L (ghostptrtoken_ty ty) (fmap f).
+  Proof.
+    move=> Rl. split; iIntros (???[|]) "*% LFT E L token //=".
+    - iDestruct "token" as (?[->->]) "[↦tys †]". iIntros "!>!>!>".
+      rewrite trans_big_sepM_mt_ty_own. iDestruct "↦tys" as (?) "[↦ tys]".
+      iMod (real_big_sepL_ty_own with "LFT E L tys") as "Upd"; [done..|].
+      iApply (step_fupdN_wand with "Upd"). iIntros "!> >(%Eq &$&?) !>".
+      iSplit; last first.
+      { iExists _. iFrame "†". iSplit; [done|]. iNext.
+        rewrite trans_big_sepM_mt_ty_own. iExists _. iFrame. }
+      iPureIntro. move: Eq=> [bl Eq]. exists (list_to_map(zip (map_to_list aπm).*1 (vec_to_list bl))). fun_ext=>/= π.
+      move: (equal_f Eq π)=>/= <-.
+      rewrite 3! vec_to_list_map. rewrite vec_to_list_to_vec.
+      rewrite -list_fmap_compose. rewrite zip_to_prod_map. rewrite list_to_map_fmap.
+      unfold mapply. rewrite map_fmap_compose. rewrite list_to_map_to_list. reflexivity.
+    - iDestruct "token" as (?) "[%Bor tys]". iIntros "!>!>!>".
+      iMod (real_big_sepM_ty_shr with "LFT E L tys") as "Upd"; [done..|].
+      iIntros "!>!>". iApply (step_fupdN_wand with "Upd").
+      iIntros ">(%Eq &$& tys) !>". iSplit; [|iExists _; by iFrame].
+      iPureIntro. move: Eq=> [bl Eq]. exists bl. fun_ext=>/= π.
+      move: (equal_f Eq π)=>/= <-.  by rewrite Bor.
+  Qed.
+
+  Lemma token_subtype {𝔄 𝔅} (f: 𝔄 → 𝔅) ty ty' E L :
+    subtype E L ty ty' f → subtype E L (ghostptrtoken_ty ty) (ghostptrtoken_ty ty') (fmap f).
+  Proof.
+    iIntros (Sub ?) "L". iDestruct (Sub with "L") as "#Sub". iIntros "!> E".
+    iDestruct ("Sub" with "E") as "(%EqSz &?&#Own&#Shr)".
+    have Eq: ∀(aπm: gmap loc (proph 𝔄)), fmap f ∘ mapply aπm = mapply (fmap (f ∘.) aπm).
+    { move=> ?. fun_ext=>/= ?. f_equal. unfold mapply. rewrite -2! map_fmap_compose. reflexivity. }
+    do 2 (iSplit; [done|]). iSplit; iIntros "!>" (?[|]) "* token //=".
+    - iDestruct "token" as (?[->->]) "(↦tys & †)". iExists  _.
+      iSplit; [done|]. rewrite 2! big_opM_fmap. rewrite EqSz.
+      iFrame "†".
+      iNext.
+      iApply (big_sepM_impl with "↦tys").
+      iModIntro. iIntros (???) "↦tys". iDestruct "↦tys" as (?) "(↦&tys)". iExists vl.
+      iFrame. iApply ("Own" with "tys").
+    - iDestruct "token" as (?->) "↦". iExists _. rewrite Eq.
+      iSplit; [done|].
+      rewrite big_opM_fmap. iApply (big_sepM_impl with "↦").
+      do 2 iModIntro. iIntros (???) "↦". iApply ("Shr" with "↦").
+  Qed.
+  Lemma token_eqtype {𝔄 𝔅} (f: 𝔄 → 𝔅) g ty ty' E L :
+    eqtype E L ty ty' f g → eqtype E L (ghostptrtoken_ty ty) (ghostptrtoken_ty ty') (fmap f) (fmap g).
+  Proof. move=> [??]. split; by apply token_subtype. Qed.
+
+  (* Rust's GhostPtrToken::new *)
+  Definition ghostptrtoken_new: val :=
+    fn: [] :=
+      let: "r" := new [ #0] in
+      let: "dummy" := new [ #0] in
+      return: ["r"].
+
+  Lemma ghostptrtoken_new_type {𝔄} (ty: type 𝔄) :
+    typed_val ghostptrtoken_new (fn(∅) → ghostptrtoken_ty ty) (λ post _, post ∅).
+  Proof.
+    eapply type_fn; [apply _|]=> _ ???. simpl_subst.
+    iIntros (???) "_ #TIME _ _ _ Na L C _ Obs". iMod persistent_time_receipt_0 as "⧖".
+    wp_bind (new _). iApply (wp_persistent_time_receipt with "TIME ⧖"); [done|].
+    iApply wp_new; [done..|]. iIntros "!>" (l) "[† _] ⧖". wp_seq.
+    wp_bind (new _). iApply (wp_persistent_time_receipt with "TIME ⧖"); [done|].
+    iApply wp_new; [done..|]. iIntros "!>" (l') "[†' _] ⧖".
+    do 3 wp_seq.
+    rewrite cctx_interp_singleton.
+    iApply ("C" $! [# #_] -[const ∅] with "Na L [-Obs] Obs"). iSplit; [|done].
+    iExists _, _. do 2 (iSplit; [done|]). rewrite/= freeable_sz_full split_mt_token'. 
+    iFrame "†". iNext. iExists ∅. iSplit.
+    iPureIntro. apply functional_extensionality. intros. unfold mapply. by rewrite fmap_empty.
+    rewrite heap_mapsto_vec_nil 2! big_opM_empty.
+    iSplit; [done|done].
+  Qed.
+End ghostptrtoken_basic.
+
+Global Hint Resolve token_resolve | 5 : lrust_typing.
+Global Hint Resolve token_resolve_just token_subtype token_eqtype : lrust_typing.
